theories/L2_typeStripped/compile.v
@@ -30,7 +30,6 @@ Inductive Term : Type :=
 | TLetIn     : name -> Term -> Term -> Term
 | TApp       : Term -> Term (* first arg must exist *) -> Terms -> Term
 | TConst     : string -> Term
-| TAx        : string -> Term
 | TInd       : inductive -> Term
 | TConstruct : inductive -> nat (* cnstr no *) ->
                nat (* # pars *) -> nat (* # args *) -> Term
@@ -79,7 +78,6 @@ Function strip (t:L1gTerm) : Term :=
     | L1g.compile.TApp fn arg args =>
       TApp (strip fn) (strip arg) (strips args)
     | L1g.compile.TConst nm => TConst nm
-    | L1g.compile.TAx s => TAx s
     | L1g.compile.TInd i => TInd i
     | L1g.compile.TConstruct i m np na => TConstruct i m np na
     | L1g.compile.TCase n _ mch brs => TCase n (strip mch) (stripBs brs)
@@ -188,4 +186,4 @@ Definition program_Program (p:program) : Program Term :=
   stripProgram (L1g.compile.program_Program p).
 
 Definition term_Term (e:AstCommon.environ L1gTerm) (t:term) : Term :=
-  strip (L1g.compile.term_Term e false t).
+  strip (L1g.compile.term_Term e t).
