theories/L2_typeStripped/term.v
@@ -78,7 +78,6 @@ Fixpoint print_term (t:Term) : string :=
     | TApp fn arg args =>
       "(" ++ (print_term fn) ++ " @ " ++ (print_term arg) ++ " _ " ++ ")"
     | TConst s => "[" ++ s ++ "]"
-    | TAx s => "(TAx " ++ s ++ ")"
     | TInd i => "(TIND " ++ (print_ind i) ++ ")"
     | TConstruct i n _ _ =>
       "(CSTR " ++ (print_ind i) ++ " " ++ (nat_to_string n) ++ ")"
@@ -114,7 +113,6 @@ Proof.
   - induction t2; cross.
     destruct (H t2_1); destruct (H0 t2_2); destruct (H1 t2); [lft | rght ..].
   - induction t; cross. destruct (string_dec s s0); [lft | rght].
-  - destruct t; cross. destruct (string_dec s s0); [lft | rght].
   - induction t; cross. destruct (inductive_dec i i0); [lft | rght].
   - induction t; cross.
     destruct (inductive_dec i i0), (eq_nat_dec n n2),
@@ -239,6 +237,20 @@ Proof.
   try (right; intros h; destruct h as [x jx]; discriminate).
   - left. auto.
 Defined.
+
+Definition isInd (t:Term) : Prop :=
+  exists i, t = TInd i.
+Lemma IsInd: forall i, isInd (TInd i).
+intros. exists i. reflexivity.
+Qed.
+Hint Resolve IsInd.
+
+Lemma isInd_dec: forall t, isInd t \/ ~ isInd t.
+Proof.
+  destruct t;
+  try (right; intros h; destruct h as [x0 j]; discriminate).
+  - left. auto.
+Qed.
 
 Definition isConstruct (t:Term) : Prop :=
   exists i n np na, t = TConstruct i n np na.
@@ -814,8 +826,6 @@ Proof.
       * apply tIn_tappend1.
   - exists (TConst s), arg, tnil. split. reflexivity.
     left. intuition. revert H. not_isApp.
-  - exists (TAx s), arg, tnil. split. reflexivity.
-    left. intuition. revert H. not_isApp.
   - exists (TInd i), arg, tnil. split. reflexivity.
     left. intuition. revert H. not_isApp.
   - exists (TConstruct i n n0 n1), arg, tnil. split. reflexivity.
@@ -841,7 +851,6 @@ Inductive WFapp: Term -> Prop :=
            ~ (isApp fn) -> WFapp fn -> WFapp t -> WFapps ts ->
            WFapp (TApp fn t ts)
 | wfaConst: forall nm, WFapp (TConst nm)
-| wfaAx: forall s, WFapp (TAx s)
 | wfaInd: forall i, WFapp (TInd i)
 | wfaConstruct: forall i m1 np na, WFapp (TConstruct i m1 np na)
 | wfaCase: forall m mch brs,
@@ -990,7 +999,6 @@ Inductive WFTrm: Term -> nat -> Prop :=
            ~ (isApp fn) -> WFTrm fn n -> WFTrm t n -> WFTrms ts n ->
            WFTrm (TApp fn t ts) n
 | wfConst: forall n nm, WFTrm (TConst nm) n
-| wfAx: forall n t, WFTrm (TAx  t) n
 | wfInd: forall n i, WFTrm (TInd i) n
 | wfConstruct: forall n i m np na, WFTrm (TConstruct i m np na) n
 | wfCase: forall n m mch brs,
@@ -1312,7 +1320,6 @@ Inductive Instantiate: nat -> Term -> Term -> Prop :=
        Instantiate n t it -> Instantiate n a ia -> Instantiates n ts its ->
        Instantiate n (TApp t a ts) (mkApp it (tcons ia its))
 | IConst: forall n s, Instantiate n (TConst s) (TConst s)
-| IAx: forall n s, Instantiate n (TAx s) (TAx s)
 | IInd: forall n ind, Instantiate n (TInd ind) (TInd ind)
 | IConstruct: forall n ind m1 np na,
        Instantiate n (TConstruct ind m1 np na) (TConstruct ind m1 np na)
