theories/L2k_noCnstrParams/compile.v
@@ -29,7 +29,6 @@ Inductive Term : Type :=
 | TLetIn     : name -> Term -> Term -> Term
 | TApp       : Term -> Term (* first arg must exist *) -> Terms -> Term
 | TConst     : string -> Term
-| TAx        : L2Term -> Term  (* L2Term is just a comment! *)
 (* constructors fully applied: eta expand *)
 | TConstruct : inductive -> nat (* cnstr no *) -> Terms (* args *) -> Term
 | TCase      : inductive -> Term (* discriminee *) ->
@@ -276,16 +275,22 @@ Functional Scheme etaExpand_args_ind :=
                                       
 (* strip params, eta expand as required,
 ** then call etaExpand_args on remaining args *)
+Function nLambda (n:nat) (F:Terms -> Term) :=
+  match n with
+  | 0 => F
+  | S m => fun b => TLambda nAnon (F b)
+  end.
+
 Function etaExpand
-         (body:Terms -> Term) (computedArgs:Terms)  (* accumulators *)
+         (body:Terms -> Term)  (* accumulator *)
          (actualArgs:Terms) (npars nargs:nat)  (* inputs *) : Term :=
   match actualArgs, npars with
   (* drop an actual arg and reduce param count *)
-  | tcons u us, S n => etaExpand (fun b => body b) tnil us n nargs
+  | tcons u us, S n => etaExpand body us n nargs
   (* no more actual args, but more params exprcted *)
-  | tnil, S n => etaExpand (fun b => TLambda nAnon (body b)) tnil tnil n nargs
-  (* keep an actual arg and reduce arg count *)
-  | aa, 0 => etaExpand_args nargs aa body computedArgs
+  | tnil, S n => etaExpand (fun b => TLambda nAnon (body b)) tnil n nargs
+  (* no more params expected; start on args *)
+  | aa, 0 => etaExpand_args nargs aa body tnil
   end.
 Functional Scheme etaExpand_ind := Induction for etaExpand Sort Prop.
 
@@ -303,14 +308,13 @@ Function strip (t:L2Term) : Term :=
     match fn with
     | L2.compile.TConstruct i m npars nargs =>
       let F := fun b => TConstruct i m b in
-      etaExpand F tnil (tcons sarg sargs) npars nargs
+      etaExpand F (tcons sarg sargs) npars nargs
     | _ => TApp (strip fn) sarg sargs
     end
   | L2.compile.TConst nm => TConst nm
-  | L2.compile.TAx s => TAx (L2.compile.TConst s)
   | L2.compile.TInd i => TDummy
   | L2.compile.TConstruct i m npars nargs =>
-    etaExpand (fun b => TConstruct i m b) tnil tnil npars nargs
+    etaExpand (fun b => TConstruct i m b) tnil npars nargs
   | L2.compile.TCase (i,_) mch brs => TCase i (strip mch) (stripBs brs)
   | L2.compile.TFix ds n => TFix (stripDs ds) n
   | L2.compile.TWrong => TWrong
