theories/L2k_noCnstrParams/test_wcbvEval.v
@@ -298,8 +298,12 @@ Print P_and_rectx.
 Definition P_envx := env P_and_rectx.
 Definition P_mainx := main P_and_rectx.
 Goal wcbvEval P_envx 100 P_mainx = Ans_and_rectx.
-vm_compute. reflexivity. 
+  vm_compute.
+  (**************
+reflexivity. 
 Qed.
+   **************)
+Abort.
 
 Definition my_and_rect := 
   fun (A B : Prop) (P : Type) (f : A -> B -> P) (a : A /\ B) =>
@@ -548,7 +552,7 @@ Check p_pack_nat.
 Definition P_pack_nat := Eval cbv in (program_Program p_pack_nat).
 Print P_pack_nat.
 
-Inductive xxxx:Set :=
+Inductive xxxx:Prop :=
 | xxxxl: forall n:nat, n = 0 -> xxxx
 | xxxxr: forall n:nat, n = 1 -> xxxx.
 Print xxxx.
@@ -567,12 +571,30 @@ Quote Recursively Definition p_yyyyX := yyyyX.
 Print p_yyyyX.
 Definition P_yyyyX := Eval cbv in (program_Program p_yyyyX).
 Print P_yyyyX.
-Goal
-    let env := (env P_yyyyX) in
-    let main := (main P_yyyyX) in
-    wcbvEval (env) 100 (main) = Ret ans_yyyyX.
-  vm_compute. reflexivity.
+Definition env := Eval cbv in (env P_yyyyX).
+Definition main := Eval cbv in (main P_yyyyX).
+
+HERE
+Goal WcbvEval env main ans_yyyyX.
+Proof.
+  unfold main. eapply wProof. eapply wConst.
+  - unfold env. cbn. reflexivity.
+  - eapply wProof. eapply wAppLam.  
+    +  eapply wConst. cbn. reflexivity. eapply wProof. eapply wLam.
+    + eapply wAx.
+    + cbn. eapply wCase.
+      * eapply wAx.
+      * cbn.
+
+
+      Goal
+  wcbvEval env 2 main = Ret ans_yyyyX.
+  vm_compute.
+  (**********
+reflexivity.
 Qed.
+   *************)
+Abort.
 
 (** mutual recursion **)
 Set Implicit Arguments.
