theories/L2_5_box/compile.v
@@ -156,7 +156,6 @@ Function L2kTerm_Term (t:L2kTerm) : Term :=
       end
     | L2k.compile.TFix defs m => TFix (L2kDefs_Defs defs) m
     | L2k.compile.TDummy => TProof
-    | L2k.compile.TAx _ => TWrong
     | L2k.compile.TWrong => TWrong
   end
 with L2kTerms_Terms (ts:L2kTerms) : Terms :=
