theories/L2_typeStripped/program.v
@@ -96,7 +96,6 @@ Inductive Crct: environ Term -> nat -> Term -> Prop :=
              Crct p n (TApp fn a args)
 | CrctConst: forall n p pd nm,
                Crct p n prop -> LookupDfn nm p pd -> Crct p n (TConst nm)
-| CrctAx: forall n p s, Crct p n prop -> Crct p n (TAx s)
 | CrctConstruct: forall n p ipkgNm inum cnum np na ipkg itp cstr pars,
                    Crct p n prop ->
                    LookupTyp ipkgNm p pars ipkg ->
@@ -374,7 +373,6 @@ Proof.
     inversion H1.
     + rewrite H6 in j. nreflexivity j.
     + eassumption.
-  - eapply CrctAx. eapply H0; try eassumption. intros h. inversion h. 
   - eapply CrctConstruct; try eassumption.
     + eapply H0. eapply H4. intros h. inversion h.
     + rewrite H4 in H1.
@@ -720,7 +718,6 @@ Proof.
     + destruct H3 as [x [h1 h2]]. eapply (@CrctConst _ _ x); trivial.
       * eapply Crct_Sort. eassumption.
   - constructor. eapply Crct_Sort. eassumption.
-  - apply CrctInd. eapply Crct_Sort. eassumption.
   - destruct ind. edestruct (Crct_invrt_Construct H0).
     + reflexivity.
     + destruct H3 as [npars [ip [h1 [it [h2 [ctr h3]]]]]].
