theories/L2k_noCnstrParams/wNorm.v
@@ -24,7 +24,6 @@ Variable p:environ Term.
 Inductive WNorm: Term -> Prop :=
 | WNLam: forall nm bod, WNorm (TLambda nm bod)
 | WNFix: forall ds br, WNorm (TFix ds br)
-| WNAx: forall t, WNorm (TAx t)
 | WNCase: forall mch n brs,
             WNorm mch -> ~ isCanonical mch ->
             WNorm (TCase n mch brs)
